finished backwards proof

theories/FOL/Util/Definability.v
@@ -1,4 +1,4 @@
-(* * Conservativity *)
+(** * Conservativity *)
 
 From Undecidability Require Import FOL.Util.FullTarski FOL.Util.Syntax FOL.Util.FullDeduction FOL.ZF.
 From Undecidability Require Import Shared.ListAutomation.
@@ -81,7 +81,7 @@ Definition is_power (x t : term') :=
   ∀ $0 ∈ t`[↑] <--> sub' $0 x`[↑].
 
 Definition is_sigma (x t : term') :=
-  ∀ $0 ∈ t`[↑] <--> $0 ≡ x`[↑] ∨ $0 ∈ x`[↑].
+  ∀ $0 ∈ t`[↑] <--> $0 ∈ x`[↑] ∨ $0 ≡ x`[↑].
 
 Definition is_inductive (t : term') :=
   (∃ is_eset $0 ∧ $0 ∈ t`[↑]) ∧ ∀ $0 ∈ t`[↑] --> (∃ is_sigma $1 $0 ∧ $0 ∈ shift 2 t).
@@ -89,236 +89,11 @@ Definition is_inductive (t : term') :=
 Definition is_om (t : term') :=
   is_inductive t ∧ ∀ is_inductive $0 --> sub' t`[↑] $0.
 
-(*Lemma eset_def {T} {HB : bounded_theory T} {HT : ZF_extension T} t :
-  ZF_tequiv T t ∅ <-> T ⊩IE is_eset t.
-Proof.
-  split; intros H.
-  - unfold is_eset. apply bt_all. intros x. cbn. asimpl.
-    fold (mem x t). rewrite H. now apply ZF_eset'.
-  - apply ZF_ext'; trivial.
-    + apply bt_all. intros x. cbn. asimpl. apply prv_T_impl.
-      apply prv_T_exf. eapply prv_T_mp; try apply prv_T1.
-      eapply prv_T_AllE in H. cbn in H. asimpl in H. apply (Weak_T H). apply tsubs_extend.
-    + apply bt_all. intros x. cbn. asimpl. apply prv_T_impl.
-      apply prv_T_exf. eapply prv_T_mp; try apply prv_T1. apply ZF_eset'. repeat solve_tsub.
-Qed.
-
-Lemma is_eset_subst t sigma :
-  (is_eset t)[sigma] = is_eset t[sigma].
-Proof.
-  unfold is_eset. cbn. asimpl. reflexivity.
-Qed.
-
-Lemma pair_def {T} {HB : bounded_theory T} {HT : ZF_extension T} x y t :
-  ZF_tequiv T t ({x; y}) <-> T ⊩IE is_pair x y t.
-fProof.
-  split; intros H.
-  - unfold is_pair. apply bt_all. intros z. cbn. asimpl. fold (mem z t). rewrite H.
-    apply prv_T_CI; apply prv_T_impl; apply ZF_pair_el'; try apply prv_T1; solve_tsub.
-  - apply ZF_ext'; trivial; apply bt_all; intros z.
-    all: apply (prv_T_AllE z) in H; cbn in *; asimpl in *.
-    + eapply prv_T_imps. eapply prv_T_CE1, H. apply prv_T_impl, ZF_pair_el', prv_T1. solve_tsub.
-    + eapply prv_T_imps'. eapply prv_T_CE2, H. apply prv_T_impl, ZF_pair_el', prv_T1. solve_tsub.
-Qed.
-
-Lemma is_pair_subst x y t sigma :
-  (is_pair x y t)[sigma] = is_pair x[sigma] y[sigma] t[sigma].
-Proof.
-  unfold is_pair. cbn. asimpl. reflexivity.
-Qed.
-
-Lemma union_def {T} {HB : bounded_theory T} {HT : ZF_extension T} x t :
-  ZF_tequiv T t (⋃ x) <-> T ⊩IE is_union x t.
-Proof.
-  split; intros H.
-  - unfold is_pair. apply bt_all. intros z. cbn. asimpl. fold (mem z t). rewrite H.
-    assert (HU : T ⊩IE ax_union). apply elem_prv. apply HT. right. tauto.
-    eapply (prv_T_AllE x) in HU. cbn in HU. eapply (prv_T_AllE z) in HU. cbn in HU.
-    asimpl in HU. apply HU.
-  - apply ZF_ext'; trivial; apply bt_all; intros z.
-    all: apply (prv_T_AllE z) in H; cbn in *; asimpl in *.
-    + eapply prv_T_imps. eapply prv_T_CE1, H. apply prv_T_impl. 
-      assert1 H'. use_exists H' y. clear H'. cbn. asimpl.
-      eapply ZF_union_el'; try apply prv_T1. repeat solve_tsub.
-    + eapply prv_T_imps'. eapply prv_T_CE2, H.
-      assert (H' : T ⊩IE ax_union). apply elem_prv. apply HT. right. tauto.
-      apply (prv_T_AllE x) in H'. cbn in H'.
-      apply (prv_T_AllE z) in H'. cbn in H'.
-      asimpl in H'. now apply prv_T_CE1 in H'.
-Qed.
-
-Lemma is_union_subst x t sigma :
-  (is_union x t)[sigma] = is_union x[sigma] t[sigma].
-Proof.
-  unfold is_union. cbn. asimpl. reflexivity.
-Qed.
-
-Lemma ZF_power {T} x y :
-  ZF ⊑ T -> T ⊩IE x ∈ PP y <-> T ⊩IE sub x y.
-Proof.
-  intros HT; split; intros H; eapply prv_T_mp; try apply H.
-  all: assert (HP : T ⊩IE ax_power) by (apply elem_prv; firstorder).
-  all: apply (prv_T_AllE y), (prv_T_AllE x) in HP; cbn in HP; asimpl in HP.
-  - eapply prv_T_CE1. apply HP.
-  - eapply prv_T_CE2. apply HP.
-Qed.
-
-Lemma ZF_sub_power {T} {HB : bounded_theory T} {HT : ZF_extension T} x y :
-  ZF_tequiv T x y -> T ⊩IE sub (PP x) (PP y).
-Proof.
-  intros H. apply bt_all. intros z. cbn. asimpl. apply prv_T_impl.
-  apply ZF_power. solve_tsub. change (T ⋄ (z ∈ PP x) ⊩IE sub z y). eapply prv_proper.
-  eapply sub_proper; eauto. reflexivity. symmetry. apply (Weak_T H).
-  repeat solve_tsub. apply ZF_power; try apply prv_T1. solve_tsub.
-Qed.
-
-Lemma ZF_eq_power {T} {HB : bounded_theory T} {HT : ZF_extension T} x y :
-  ZF_tequiv T x y -> T ⊩IE PP x ≡ PP y.
-Proof.
-  intros H. apply ZF_ext'; trivial; now apply ZF_sub_power.
-Qed.
-
-Lemma sub_subst x y sigma :
-  (sub x y)[sigma] = sub x[sigma] y[sigma].
-Proof.
-  cbn. unfold sub, shift. asimpl. reflexivity.
-Qed.
-
-Lemma power_def {T} {HB : bounded_theory T} {HT : ZF_extension T} x t :
-  ZF_tequiv T t (PP x) <-> T ⊩IE is_power x t.
-Proof.
-  split; intros H.
-  - unfold is_power. apply bt_all. intros y. cbn. asimpl. fold (mem y t). rewrite H.
-    apply prv_T_CI; apply prv_T_impl; apply ZF_power; try apply prv_T1; solve_tsub.
-  - apply ZF_ext'; trivial; apply bt_all; intros z.
-    all: apply (prv_T_AllE z) in H;  cbn -[sub] in *.
-    all: setoid_rewrite sub_subst in H; cbn in H; asimpl in H.
-    + eapply prv_T_imps. eapply prv_T_CE1, H. apply prv_T_impl, ZF_power, prv_T1. solve_tsub.
-    + eapply prv_T_imps'. eapply prv_T_CE2, H. apply prv_T_impl, ZF_power, prv_T1. solve_tsub.
-Qed.
-
-Lemma is_power_subst x t sigma :
-  (is_power x t)[sigma] = is_power x[sigma] t[sigma].
-Proof.
-  unfold is_power, sub. cbn. asimpl. reflexivity.
-Qed.
-
-Lemma inductive_subst x sigma :
-  (inductive x)[sigma] = inductive x[sigma].
-Proof.
-  cbn. unfold inductive. cbn. asimpl. reflexivity.
-Qed.
-
-Lemma ZF_om1 {T} {HT : ZF_extension T} :
-  T ⊩IE inductive ω.
-Proof.
-  apply elem_prv. apply HT. right. tauto.
-Qed.
-
-Lemma ZF_om2 {T} {HT : ZF_extension T} x :
-  T ⊩IE inductive x -> T ⊩IE sub ω x.
-Proof.
-  intros H. eapply prv_T_mp. 2: apply H.
-  assert (H' : T ⊩IE ax_om2). apply elem_prv, HT. right. tauto.
-  apply (prv_T_AllE x) in H'. cbn -[inductive sub] in H'.
-  setoid_rewrite sub_subst in H'. now setoid_rewrite inductive_subst in H'.
-Qed.
-
-Lemma ZF_sigma_el {T} {HT : ZF_extension T} x y :
-  T ⊩IE x ∈ σ y <-> T ⊩IE x ≡ y ∨ x ∈ y.
-Proof.
-  split; intros H.
-  - eapply prv_T_mp; try apply H. apply bunion_use; trivial.
-    + apply prv_T_DI2, prv_T1.
-    + apply prv_T_DI1, prv_T1. 
-  - apply ZF_bunion_el'; trivial. apply (prv_T_DE H).
-    + apply prv_T_DI2. eapply ZF_sing_iff, prv_T1. solve_tsub.
-    + apply prv_T_DI1, prv_T1.
-Qed.
-
-Lemma sigma_def {T} {HB : bounded_theory T} {HT : ZF_extension T} x t :
-  ZF_tequiv T t (σ x) <-> T ⊩IE is_sigma x t.
-Proof.
-  split; intros H.
-  - unfold is_sigma. apply bt_all. intros z. cbn. asimpl. fold (mem z t). rewrite H.
-    apply prv_T_CI; apply prv_T_impl; apply ZF_sigma_el; try apply prv_T1; solve_tsub.
-  - apply ZF_ext'; trivial; apply bt_all; intros z.
-    all: apply (prv_T_AllE z) in H; cbn in *; asimpl in *.
-    + eapply prv_T_imps. eapply prv_T_CE1, H. apply prv_T_impl, ZF_sigma_el, prv_T1.
-    + eapply prv_T_imps'. eapply prv_T_CE2, H. apply prv_T_impl, ZF_sigma_el, prv_T1.
-Qed.
-
-Lemma is_sigma_subst x t sigma :
-  (is_sigma x t)[sigma] = is_sigma x[sigma] t[sigma].
-Proof.
-  unfold is_sigma. cbn. asimpl. reflexivity.
-Qed.
-
-Lemma is_inductive_subst x sigma :
-  (is_inductive x)[sigma] = is_inductive x[sigma].
-Proof.
-  cbn. unfold is_inductive. cbn. asimpl. reflexivity.
-Qed.
-
-Lemma is_inductive_spec {T} {HB : bounded_theory T} {HT : ZF_extension T} x :
-  T ⊩IE is_inductive x <-> T ⊩IE inductive x.
-Proof.
-  split; intros H.
-  - apply prv_T_CI.
-    + apply prv_T_CE1 in H. use_exists H y. clear H.
-      cbn -[is_eset]. asimpl. setoid_rewrite is_eset_subst. cbn.
-      assert1 H. apply prv_T_CE in H as [H1 H2]. apply eset_def in H1.
-      fold (mem ∅ x). now rewrite <- H1.
-    + apply bt_all. intros y. cbn. asimpl. apply prv_T_CE2, (prv_T_AllE y) in H.
-      cbn -[is_sigma] in H. asimpl in H. apply (prv_T_imps H), prv_T_impl. clear H.
-      assert1 H. use_exists H z. clear H. apply prv_clear2. cbn -[is_sigma]. asimpl.
-      setoid_rewrite is_sigma_subst. cbn. assert1 H. apply prv_T_CE in H as [H1 H2].
-      apply sigma_def in H1. fold (mem (σ y) x). now rewrite <- H1.
-  - apply prv_T_CI.
-    + eapply prv_T_ExI. cbn -[is_eset]. asimpl. apply prv_T_CI.
-      * setoid_rewrite is_eset_subst. cbn. now apply eset_def, ZF_refl'.
-      * eapply prv_T_CE1, H.
-    + apply bt_all. intros y. cbn -[is_sigma]. asimpl.
-      apply prv_T_CE2, (prv_T_AllE y) in H.
-      eapply prv_T_impl, prv_T_ExI. cbn -[is_sigma]. apply prv_T_CI.
-      * rewrite is_sigma_subst. cbn. asimpl. apply sigma_def, ZF_refl'. solve_tsub.
-      * asimpl. cbn in H. asimpl in H. now apply prv_T_imp.
-Qed.
-
-Lemma om_def {T} {HB : bounded_theory T} {HT : ZF_extension T} t :
-  ZF_tequiv T t ω <-> T ⊩IE is_om t.
-Proof.
-  split; intros H.
-  - unfold is_om. apply prv_T_CI. apply prv_T_CI.
-    + eapply prv_T_ExI. cbn -[is_eset]. asimpl. apply prv_T_CI.
-      * setoid_rewrite is_eset_subst. cbn. now apply eset_def, ZF_refl'.
-      * fold (mem ∅ t). rewrite H. eapply prv_T_CE1. apply ZF_om1.
-    + apply bt_all. intros x. cbn -[is_sigma]. asimpl. fold (mem x t) (mem (σ x) t).
-      rewrite H at 1. pose proof ZF_om1 as H'. apply prv_T_CE2, (prv_T_AllE x) in H'.
-      eapply prv_T_impl, prv_T_ExI. cbn -[is_sigma]. apply prv_T_CI.
-      * rewrite is_sigma_subst. cbn. asimpl. apply sigma_def, ZF_refl'. solve_tsub.
-      * asimpl. cbn in H'. apply prv_T_imp. fold (mem (σ x) t). now rewrite H.
-    + apply bt_all. intros x. cbn -[is_inductive sub].
-      setoid_rewrite sub_subst. setoid_rewrite is_inductive_subst. cbn. asimpl.
-      apply prv_T_impl. eapply prv_proper. eapply sub_proper; eauto. apply (Weak_T H).
-      repeat solve_tsub. reflexivity. apply ZF_om2, is_inductive_spec, prv_T1.
-  - apply ZF_ext'; trivial.
-    + eapply prv_T_CE2, (prv_T_AllE) in H. cbn -[is_inductive sub] in H. asimpl in H.
-      setoid_rewrite sub_subst in H. setoid_rewrite is_inductive_subst in H.
-      cbn in H. asimpl in H. apply (prv_T_mp H). now apply is_inductive_spec, ZF_om1.
-    + apply ZF_om2, is_inductive_spec. now apply prv_T_CE1 in H.
-Qed.
-
-Lemma is_om_subst t sigma :
-  (is_om t)[sigma] = is_om t[sigma].
-Proof.
-  unfold is_om, is_inductive, sub. cbn. asimpl. reflexivity.
-Qed. *)
 
 
 (** Translation function *)
 
-Definition sshift k : nat -> term' :=
+Definition sshift {Σ_funcs : funcs_signature} k : nat -> term :=
   fun n => match n with 0 => $0 | S n => $(1 + k + n) end.
 
 Fixpoint rm_const_tm (t : term) : form' :=
@@ -333,27 +108,6 @@ Fixpoint rm_const_tm (t : term) : form' :=
   | func power v => ∃ (Vector.hd (Vector.map rm_const_tm v))[sshift 1] ∧ is_power $0 $1
   | func omega v => is_om $0
   end.
-
-Lemma form_full_rect {Σ_funcs : funcs_signature} {Σ_preds : preds_signature} {ops : operators}
-         (P : form falsity_on -> Type) :
-       P ⊥ ->
-       (forall (P0 : Σ_preds) (t : Vector.t term (ar_preds P0)), P (atom _ _ _ falsity_on P0 t)) ->
-       (forall (b0 : binop) (f1 : form falsity_on), P f1 -> forall f2 : form falsity_on, P f2 -> P (bin b0 f1 f2)) ->
-       (forall (q : quantop) (f2 : form falsity_on), P f2 -> P (quant q f2)) ->
-       forall(f4 : form falsity_on), P f4.
-Proof.
-Admitted.
-
-Definition rm_const_fm' (phi : form) : form'.
-Proof.
-  revert phi. apply form_full_rect.
-  - exact ⊥.
-  - intros [] v; pose (v' := Vector.map rm_const_tm v).
-    + exact (∃ (Vector.hd v') ∧ ∃ (Vector.hd (Vector.tl v'))[sshift 1] ∧ $1 ∈ $0).
-    + exact (∃ (Vector.hd v') ∧ ∃ (Vector.hd (Vector.tl v'))[sshift 1] ∧ $1 ≡ $0).
-  - intros bop phi phi' psi psi'. exact (bin bop phi' psi').
-  - intros qop phi phi'. exact (quant qop phi').
-Defined.
 
 Fixpoint rm_const_fm {ff : falsity_flag} (phi : form) : form' :=
   match phi with
@@ -393,13 +147,13 @@ Qed.
 Hint Rewrite map_hd map_tl : vecs.
 
 Lemma in_hd X n (v : vec X (S n)) :
-  vec_in (Vector.hd v) v.
+  Vector.In (Vector.hd v) v.
 Proof.
   depelim v. constructor.
 Qed.
 
 Lemma in_hd_tl X n (v : vec X (S (S n))) :
-  vec_in (Vector.hd (Vector.tl v)) v.
+  Vector.In (Vector.hd (Vector.tl v)) v.
 Proof.
   depelim v. constructor. depelim v. constructor.
 Qed.
@@ -468,10 +222,83 @@ Section Model.
       unfold funcomp. cbn. unfold funcomp. now destruct (sigma n) as [x|[]].
   Qed.
 
+  Lemma embed_sshift n (phi : form') :
+    embed phi[sshift n] = (embed phi)[sshift n].
+  Proof.
+    rewrite embed_subst. apply subst_ext. now intros [].
+  Qed.
+
+  Lemma sat_sshift1 (rho : nat -> V) x y (phi : form) :
+    (y .: x .: rho) ⊨ phi[sshift 1] <-> (y .: rho) ⊨ phi.
+  Proof.
+    erewrite sat_comp, sat_ext. reflexivity. now intros [].
+  Qed.
+
+  Lemma sat_sshift2 (rho : nat -> V) x y z (phi : form) :
+    (z .: y .: x .: rho) ⊨ phi[sshift 2] <-> (z .: rho) ⊨ phi.
+  Proof.
+    erewrite sat_comp, sat_ext. reflexivity. now intros [].
+  Qed.
+
   Lemma rm_const_tm_sat (rho : nat -> V) (t : term) x :
     (x .: rho) ⊨ embed (rm_const_tm t) <-> x = eval rho t.
   Proof.
-  Admitted.
+    induction t in x |- *; try destruct F; cbn; split; try intros ->;
+    autorewrite with vecs in *; try rewrite (vec_inv1 v); try rewrite (vec_inv2 v); cbn.
+    - now rewrite VIEQ.
+    - now rewrite VIEQ.
+    - cbn in v. rewrite (vec_nil_eq (Vector.map (eval rho) v)).
+      intros H. apply M_ext; trivial; intros y Hy; exfalso; intuition.
+      now apply M_eset in Hy. 
+    - cbn in v. rewrite (vec_nil_eq (Vector.map (eval rho) v)).
+      intros d. now apply M_eset.
+    - intros (y & Hy & z & Hz & H).
+      rewrite embed_sshift, sat_sshift1, IH in Hy; try apply in_hd. subst.
+      rewrite embed_sshift, sat_sshift2, IH in Hz; try apply in_hd_tl. subst.
+      apply M_ext; trivial.
+      + intros a Ha % H. rewrite !VIEQ in Ha. now apply M_pair.
+      + intros a Ha % M_pair; trivial. apply H. now rewrite !VIEQ.
+    - exists (eval rho (Vector.hd v)).
+      rewrite embed_sshift, sat_sshift1, IH; try apply in_hd. split; trivial.
+      exists (eval rho (Vector.hd (Vector.tl v))).
+      rewrite embed_sshift, sat_sshift2, IH; try apply in_hd_tl. split; trivial.
+      intros d. rewrite !VIEQ. now apply M_pair.
+    - intros (y & Hy & H).
+      rewrite embed_sshift, sat_sshift1, IH in Hy; try apply in_hd. subst.
+      apply M_ext; trivial.
+      + intros y Hy % H. now apply M_union.
+      + intros y Hy % M_union; trivial. now apply H.
+    - exists (eval rho (Vector.hd v)).
+      rewrite embed_sshift, sat_sshift1, IH; try apply in_hd. split; trivial.
+      intros d. now apply M_union.
+    - intros (y & Hy & H).
+      rewrite embed_sshift, sat_sshift1, IH in Hy; try apply in_hd. subst.
+      apply M_ext; trivial.
+      + intros y Hy. now apply M_power, H.
+      + intros y Hy. now apply H, M_power.
+    - exists (eval rho (Vector.hd v)).
+      rewrite embed_sshift, sat_sshift1, IH; try apply in_hd. split; trivial.
+      intros d. now apply M_power.
+    - cbn in v. rewrite (vec_nil_eq (Vector.map (eval rho) v)). setoid_rewrite VIEQ.
+      intros [H1 H2]. apply M_ext; trivial.
+      + apply H2. split. exists ∅. split; try apply M_eset; trivial. now apply M_om1.
+        intros d Hd. exists (σ d). split; try now apply M_om1. intros d'. now apply sigma_el.
+      + apply M_om2; trivial. split.
+        * destruct H1 as [[d Hd] _]. enough (∅ = d) as -> by apply Hd.
+          apply M_ext; trivial; intros y Hy; exfalso; intuition. now apply M_eset in Hy.
+        * intros d [d' Hd] % H1. enough (σ d = d') as -> by apply Hd. apply M_ext; trivial.
+          -- intros a Ha % sigma_el; trivial. now apply Hd.
+          -- intros a Ha % Hd. now apply sigma_el.
+    - cbn in v. rewrite (vec_nil_eq (Vector.map (eval rho) v)). setoid_rewrite VIEQ. split.
+      + split. exists ∅. split; try apply M_eset; trivial. now apply M_om1.
+        intros d Hd. exists (σ d). split; try now apply M_om1. intros d'. now apply sigma_el.
+      + intros d Hd. apply M_om2; trivial. split.
+        * destruct Hd as [[y Hy] _]. enough (∅ = y) as -> by apply Hy.
+          apply M_ext; trivial; intros z Hz; exfalso; intuition. now apply M_eset in Hz.
+        * intros y [z Hz] % Hd. enough (σ y = z) as -> by apply Hz. apply M_ext; trivial.
+          -- intros a Ha % sigma_el; trivial. now apply Hz.
+          -- intros a Ha % Hz. now apply sigma_el.
+  Qed.
 
   Lemma rm_const_sat (rho : nat -> V) (phi : form) :
     rho ⊨ phi <-> rho ⊨ embed (rm_const_fm phi).
